12

sf/Assignment12_05.v
@@ -13,32 +13,78 @@ Require Export Assignment12_04.
 *)
 
 Definition halve : tm :=
-  FILL_IN_HERE.
+  tfix (tabs Halve (TArrow TNat TNat) (tabs X (TNat) 
+  (tif0 (tvar X) (tnat 0) (tif0 (tpred (tvar X)) (tnat 0)
+  (tsucc (tapp (tvar Halve) (tpred (tpred (tvar X)))))))))
+.
 
 Example halve_type: empty |- halve \in TArrow TNat TNat.
 Proof.
-  (* unfold halve; eauto 10. *)
-  exact FILL_IN_HERE.
+  unfold halve; eauto 10.
 Qed.
 
 Example halve_10: tapp halve (tnat 10) ==>* tnat 5.
 Proof.
-  (* unfold halve; normalize. *)
-  exact FILL_IN_HERE.
+  unfold halve; normalize.
 Qed.
 
 Example halve_11: tapp halve (tnat 11) ==>* tnat 5.
 Proof.
-  (* unfold halve; normalize. *)
-  exact FILL_IN_HERE.
+  unfold halve; normalize.
+Qed.
+
+Lemma sub0: forall t t',
+  t ==>* t' -> tsucc t ==>* tsucc t'.
+Proof.
+  intros.
+  induction H.
+  constructor.
+  eapply multi_step.
+  constructor.
+  apply H.
+  apply IHmulti.
 Qed.
 
 
 Theorem halve_correct: forall n,
    tapp halve (tnat (n+n)) ==>* tnat n.
 Proof.
-  exact FILL_IN_HERE.
+  intros. unfold halve.
+  induction n.
+  simpl. eapply multi_step.
+  eauto.
+  eapply multi_step.
+  eauto.
+  eapply multi_step.
+  eapply ST_AppAbs.
+  constructor.
+  eapply multi_step. simpl.
+  eauto. constructor.
+  simpl.
+  eapply multi_step.
+  eauto.
+  eapply multi_step.
+  eauto.
+  eapply multi_step.
+  eapply ST_AppAbs.
+  constructor. simpl.
+  eapply multi_step. eauto.
+  eapply multi_step. eauto.
+  eapply multi_step. simpl.
+  assert (n + S n = S (n + n)).
+  omega. rewrite H.
+  eapply ST_If0Nonzero.
+  eapply multi_step. eauto.
+  eapply multi_step. eauto.
+  simpl.
+  apply sub0 in IHn. 
+  eapply multi_trans.
+  apply IHn.
+  eapply multi_step.
+  eauto.
+  constructor.
 Qed.
+
 
 (*-- Check --*)
 
