sf/Assignment12_01.v
@@ -8,6 +8,23 @@ Require Export Assignment12_00.
           empty |- \x:S. x x : T).
 *)
 
+Lemma typing_sub0 :
+  ~ (exists T1, exists T2, T1 = TArrow T1 T2).
+Proof.
+  intros Hc.
+  inversion Hc as [T H].
+  clear Hc.
+  induction T.
+  inversion H.
+  inversion H0.
+  apply IHT1. exists T2. apply H2.
+  inversion H. inversion H0.
+  inversion H. inversion H0.
+  inversion H. inversion H0.
+  inversion H. inversion H0.
+  inversion H. inversion H0.
+Qed.
+
 Example typing_nonexample_3 :
   ~ (exists S, exists T,
         empty |- 
@@ -15,7 +32,20 @@ Example typing_nonexample_3 :
              (tapp (tvar X) (tvar X))) \in
           T).
 Proof.
-  exact FILL_IN_HERE.
+  unfold not.
+  intros.
+  inversion H.
+  inversion H0.
+  inversion H1; subst.
+  inversion H7; subst.
+  inversion H8; subst.
+  inversion H5; subst.
+  inversion H4.
+  inversion H6.
+  rewrite H3 in H9.
+  apply typing_sub0.
+  exists T1. exists T12.
+  apply H9.
 Qed.
 
 (*-- Check --*)
