sf/Assignment12_03.v
@@ -12,8 +12,48 @@ Lemma type_is_unique: forall t G T T'
     (TYPED': G |- t \in T'),
   T = T'.
 Proof.
-  exact FILL_IN_HERE.
+  intros.
+  generalize dependent T'.
+  induction TYPED; intros.
+  inversion TYPED'; subst.
+  rewrite H in H2. inversion H2.
+  reflexivity.
+  inversion TYPED'; subst.
+  apply IHTYPED in H4. rewrite H4.
+  reflexivity.
+  inversion TYPED'; subst.
+  apply IHTYPED1 in H2.
+  apply IHTYPED2 in H4.
+  subst.
+  inversion H2.
+  reflexivity.
+  inversion TYPED'; subst. reflexivity.
+  inversion TYPED'; subst. reflexivity.
+  inversion TYPED'; subst. reflexivity.
+  inversion TYPED'; subst. reflexivity.
+  inversion TYPED'; subst.
+  apply IHTYPED2 in H5. apply H5.
+  inversion TYPED'; subst. apply IHTYPED1 in H2.
+  apply IHTYPED2 in H4. subst. reflexivity.
+  inversion TYPED'; subst. apply IHTYPED in H1. inversion H1.
+  reflexivity. inversion TYPED'; subst. apply IHTYPED in H1.
+  inversion H1. subst. reflexivity. inversion TYPED'; subst.
+  reflexivity. inversion TYPED'; subst. apply IHTYPED1 in H4.
+  subst.
+  apply IHTYPED2 in H5. apply H5.
+  inversion TYPED'; subst. apply IHTYPED in H3. subst. reflexivity.
+  inversion TYPED'; subst. apply IHTYPED in H3. subst. reflexivity.
+  inversion TYPED'; subst. apply IHTYPED1 in H6.
+  inversion H6. subst.
+  apply IHTYPED2 in H7. apply H7.
+  inversion TYPED'; subst. reflexivity.
+  inversion TYPED'; subst. apply IHTYPED2 in H4. apply H4.
+  inversion TYPED'; subst.
+  apply IHTYPED2 in H7. apply H7.
+  inversion TYPED'; subst. apply IHTYPED in H1.
+  inversion H1; subst. reflexivity.
 Qed.
+
 
 (*-- Check --*)
 Check type_is_unique: forall t G T T'
