sf/Assignment12_04.v
@@ -7,7 +7,18 @@ Corollary soundness : forall t t' T,
   t ==>* t' ->
   ~(stuck t').
 Proof.
-  exact FILL_IN_HERE.
+  unfold not. unfold stuck. unfold normal_form. unfold not.
+  intros.
+  destruct H1.
+  assert (\empty |- t \in T).
+  apply H.
+  induction H0; subst.
+  apply progress in H. inversion H. apply H2 in H0. apply H0.
+  apply H1 in H0. apply H0.
+  apply preservation with (t' := y) in H3.
+  apply IHmulti.
+  apply H3. apply H1. apply H2. apply H3.
+  apply H0.
 Qed.
 
 (*-- Check --*)
